Weidenbach_Book/CDCL_Two_Watched_Literals_Watch_List.thy
@@ -1828,28 +1828,32 @@ theorem cdcl_twl_stgy_prog_wl_spec_final2:
 
 subsection \<open>Final Theorem with Initialisation\<close>
 
-fun init_wl_of :: \<open>'v twl_st_l \<Rightarrow> 'v twl_st_wl\<close> where
+fun init_wl_of :: \<open>'v twl_st_l\<Rightarrow> 'v twl_st_wl\<close> where
   \<open>init_wl_of (M, N, U, D, NP, UP, _, Q) =
-       (M, N, U, D, NP, UP, Q, calculate_correct_watching (tl N) (\<lambda>_. []) 1)\<close>
+       ((M, N, U, D, NP, UP, Q, calculate_correct_watching (tl N) (\<lambda>_. []) 1))\<close>
+
+lemma twl_struct_invs_init_twl_struct_invs:
+  \<open>snd S = {#} \<Longrightarrow> twl_struct_invs_init S \<longleftrightarrow> twl_struct_invs (fst S)\<close>
+  by (cases S) (auto simp: twl_struct_invs_def twl_struct_invs_init_def)
 
 theorem init_dt_wl:
   fixes CS S
-  defines S\<^sub>0: \<open>S\<^sub>0 \<equiv> ([], [[]], 0, None, {#}, {#}, {#}, {#})\<close>
-  defines S: \<open>S \<equiv> init_wl_of (init_dt CS S\<^sub>0)\<close>
+  defines S\<^sub>0: \<open>S\<^sub>0 \<equiv> (([], [[]], 0, None, {#}, {#}, {#}, {#}), {#})\<close>
+  defines S: \<open>S \<equiv>  init_wl_of (fst (init_dt CS S\<^sub>0))\<close>
   assumes
     dist: \<open>\<forall>C \<in> set CS. distinct C\<close> and
-    le: \<open>\<forall>C \<in> set CS. length C \<ge> 1\<close> and
-    no_confl: \<open>get_conflict_wl S = None\<close>
+    no_confl: \<open>get_conflict_wl S = None\<close> and
+    snd_init: \<open>snd (init_dt CS S\<^sub>0) = {#}\<close>
   shows
     \<open>cdcl_twl_stgy_prog_wl S \<le> SPEC (\<lambda>T. full cdcl\<^sub>W_restart_mset.cdcl\<^sub>W_stgy
              (state\<^sub>W_of (twl_st_of_wl None S))
              (state\<^sub>W_of (twl_st_of_wl None T)))\<close>
 proof -
-  obtain M N U D NP UP WS Q where
-    init: \<open>init_dt CS S\<^sub>0 = (M, N, U, D, NP, UP, WS, Q)\<close>
+  obtain M N U D NP UP WS Q OC where
+    init: \<open>init_dt CS S\<^sub>0 = ((M, N, U, D, NP, UP, WS, Q), OC)\<close>
     by (cases \<open>init_dt CS S\<^sub>0\<close>) auto
   have \<open>N \<noteq> []\<close>
-    using clauses_init_dt_not_Nil[of CS] init unfolding S\<^sub>0[symmetric] by auto
+    using clauses_init_dt_not_Nil[of CS \<open>snd S\<^sub>0\<close>] init unfolding S\<^sub>0 by auto
   then have corr_w: \<open>correct_watching S\<close>
     unfolding S init
     by (auto simp: correct_watching.simps
@@ -1861,18 +1865,17 @@ proof -
     \<open>additional_WS_invs (st_l_of_wl None S)\<close>
     unfolding S S\<^sub>0
     subgoal
-      using init_dt(1)[OF dist le]
-        by (cases \<open>(init_dt CS ([], [[]], 0, None, {#}, {#}, {#}, {#}))\<close>) auto
+      using init_dt(1)[OF dist] snd_init
+        by (cases \<open>init_dt CS S\<^sub>0\<close>) (auto simp: S\<^sub>0 twl_struct_invs_init_twl_struct_invs)
     subgoal
-      using init_dt(2)[OF dist le]
-        by (cases \<open>(init_dt CS ([], [[]], 0, None, {#}, {#}, {#}, {#}))\<close>) auto
+      using init_dt(2)[OF dist] snd_init
+      by (cases \<open>init_dt CS S\<^sub>0\<close>) (auto simp: S\<^sub>0 clauses_def)
     subgoal
-      using init_dt(3)[OF dist le]
-        by (cases \<open>(init_dt CS ([], [[]], 0, None, {#}, {#}, {#}, {#}))\<close>) auto
+      using init_dt(3)[OF dist] snd_init
+      by (cases \<open>init_dt CS S\<^sub>0\<close>) (auto simp: S\<^sub>0 clauses_def)
     subgoal
-      using init_dt(5)[OF dist le]
-      by (cases \<open>(init_dt CS ([], [[]], 0, None, {#}, {#}, {#}, {#}))\<close>)
-        (auto simp: additional_WS_invs_def)
+      using init_dt(5)[OF dist]
+      by (cases \<open>init_dt CS S\<^sub>0\<close>) (auto simp: S\<^sub>0 clauses_def additional_WS_invs_def)
     done
   from cdcl_twl_stgy_prog_wl_spec_final2[OF this(1,3) no_confl this(4) corr_w]
   show ?thesis
